Due to the fact that  two of the  studied classes of systems that are studied in this paper are affine functions in terms of $f$ and $g$, we propose to solve the "one--step nonsmooth problem'' (\ref{eq:toto1}) by performing an external Newton linearization. \paragraph{Newton's linearization of the first line of~(\ref{eq:toto1})} The first line of the  problem~(\ref{eq:toto1}) can be written under the form of a residue $\mathcal R$ depending only on $x_{k+1}$ and $r_{k+1}$ such that \begin{equation}  \label{eq:NL3}  \mathcal R (x_{k+1},r _{k+1}) =0\end{equation}with \begin{equation}\mathcal R(x,r) = M(x - x_{k}) -h\theta f( x , t_{k+1}) - h(1-\theta)f(x_k,t_k) - h\gamma r- h(1-\gamma)r_k.\end{equation}The solution of this system of nonlinear equations is sought as a limit of the sequence $\{ x^{\alpha}_{k+1},r^{\alpha}_{k+1} \}_{\alpha \in \NN}$ such that \begin{equation}   \label{eq:NL7}   \begin{cases}     x^{0}_{k+1} = x_k \\ \\     r^{0}_{k+1} = r_k \\ \\     \mathcal R_L( x^{\alpha+1}_{k+1},r^{\alpha+1}_{k+1}) = \mathcal     R(x^{\alpha}_{k+1},r^{\alpha}_{k+1})  + \left[ \nabla_{x} \mathcal     R(x^{\alpha}_{k+1},r^{\alpha}_{k+1})\right] (x^{\alpha+1}_{k+1}-x^{\alpha}_{k+1} ) +     \left[ \nabla_{r} \mathcal R(x^{\alpha}_{k+1},r^{\alpha}_{k+1})\right] (r^{\alpha+1}_{k+1} - r^{\alpha}_{k+1} ) =0 \end{cases}\end{equation}\begin{ndrva}  What about $r^0_{k+1}$ ?\end{ndrva}The residu \free $\mathcal R _{\free}$ is also defined (useful for implementation only):\[\mathcal R _{\free}(x) \stackrel{\Delta}{=}  M(x - x_{k}) -h\theta f( x , t_{k+1}) - h(1-\theta)f(x_k,t_k),\]which yields\[\mathcal R (x,r) = \mathcal R _{\free}(x)   - h\gamma r - h(1-\gamma)r_k.\]\begin{equation}  \mathcal R (x^{\alpha}_{k+1},r^{\alpha}_{k+1}) = \fbox{$\mathcal R^{\alpha}_{k+1} \stackrel{\Delta}{=}  \mathcal R_{\free}(x^{\alpha}_{k+1})  - h\gamma r^{\alpha}_{k+1} - h(1-\gamma)r_k$}\label{eq:rfree-1}\end{equation}\[  \mathcal R_{\free}(x^{\alpha}_{k+1},r^{\alpha}_{k+1} )=\fbox{$ \mathcal R _{\free, k+1} ^{\alpha} \stackrel{\Delta}{=}  M(x^{\alpha}_{k+1} - x_{k}) -h\theta f( x^{\alpha}_{k+1} , t_{k+1}) - h(1-\theta)f(x_k,t_k)$}\] % The computation of the Jacobian of $\mathcal R$ with respect to $x$, denoted by $   W^{\alpha}_{k+1}$ leads to % \begin{equation}%    \label{eq:NL9}%    \begin{array}{l}%     W^{\alpha}_{k+1} \stackrel{\Delta}{=} \nabla_{x} \mathcal R (x^{\alpha}_{k+1},r^{\alpha}_{k+1})= M - h  \theta \nabla_{x} f(  x^{\alpha}_{k+1}, t_{k+1} ).\\%  \end{array}% \end{equation}At each time--step, we have to solve the following linearized problem,\begin{equation}   \label{eq:NL10}    \mathcal R^{\alpha}_{k+1} + (M-h\theta A ^{\alpha}_{k+1}) (x^{\alpha+1}_{k+1} -    x^{\alpha}_{k+1}) - h \gamma (r^{\alpha+1}_{k+1} - r^{\alpha}_{k+1} )  =0 ,\end{equation}with \begin{equation}     \begin{array}{l}       A^{\alpha}_{k+1} = \nabla_x f(t_{k+1}, x^{\alpha}_{k+1})  \end{array}\end{equation}By using (\ref{eq:rfree-1}), we get\begin{equation}  \label{eq:rfree-2}  \mathcal R_{\free}(x^{\alpha}_{k+1},r^{\alpha}_{k+1} )  - h\gamma r^{\alpha+1}_{k+1} - h(1-\gamma)r_k  + (M-h\theta A^{\alpha}_{k+1}) (x^{\alpha+1}_{k+1} -    x^{\alpha}_{k+1})  =0 \end{equation}% %\fbox% {%   \begin{equation}%     \label{eq:rfree-11}%     \boxed{ x^{\alpha+1}_{k+1} = h\gamma (W^{\alpha}_{k+1})^{-1}r^{\alpha+1}_{k+1} +x^\alpha_{\free}}%   \end{equation}% }% with :% \begin{equation}%   \label{eq:rfree-12}%   \boxed{x^\alpha_{\free}\stackrel{\Delta}{=}x^{\alpha}_{k+1}-(W^{\alpha}_{k+1})^{-1}\mathcal (R_{\free,k+1}^{\alpha} \textcolor{red}{- h(1-\gamma) r_k})}% \end{equation}The matrix $W$ is clearly non singular for small $h$.% that is% \begin{equation}%    \begin{array}{l}%  h \gamma  r^{\alpha+1}_{k+1} = r_c + W^{\alpha}_{k+1} x^{\alpha+1}_{k+1}%  .\label{eq:NL11} %  \end{array}% \end{equation}% with % \begin{equation}%    \begin{array}{l}% r_c \stackrel{\Delta}{=} h \gamma r^{\alpha}_{k+1} - W^{\alpha}_{k+1} x^{\alpha}_{k+1} + \mathcal R% ^{\alpha}_{k+1}=- W^{\alpha}_{k+1} x^{\alpha}_{k+1} + \mathcal R_{\free k+1} ^{\alpha} - h(1-\gamma)r_k\\ \\% \end{array}% \end{equation}% \begin{equation}%    \begin{array}{l}% \mathcal R ^{\alpha}_{k+1}=M( x^{\alpha}_{k+1} - x_k) -h \theta f(x^{\alpha}_{k+1})-h(1-\theta)f(x_k)% - h \gamma r^{\alpha}_{k+1} -h(1- \gamma)r_k%  \end{array}%    \end{equation}% \[x^{\alpha+1}_{k+1} = h(W^{\alpha}_{k+1})^{-1}r^{\alpha+1}_{k+1} +(W^{\alpha}_{k+1})^{-1}(\mathcal% R_{\free k+1} ^{\alpha})+x^{\alpha}_{k+1}\] \paragraph{Newton's linearization of the second  line of~(\ref{eq:toto1})}The same operation is performed with the second equation of (\ref{eq:toto1})\begin{equation}  \begin{array}{l}    \mathcal R_y(x,y,\lambda)=y-h(t_{k+1},x,\lambda) =0\\ \\  \end{array}\end{equation}which is linearized as\begin{equation}  \label{eq:NL9}  \begin{array}{l}    \mathcal R_{Ly}(x^{\alpha+1}_{k+1},y^{\alpha+1}_{k+1},\lambda^{\alpha+1}_{k+1}) = \mathcal    R_{y}(x^{\alpha}_{k+1},y^{\alpha}_{k+1},\lambda^{\alpha}_{k+1}) +    (y^{\alpha+1}_{k+1}-y^{\alpha}_{k+1})- \\[2mm] \qquad  \qquad \qquad \qquad  \qquad \qquad    C^{\alpha}_{k+1}(x^{\alpha+1}_{k+1}-x^{\alpha}_{k+1}) - D^{\alpha}_{k+1}(\lambda^{\alpha+1}_{k+1}-\lambda^{\alpha}_{k+1})=0  \end{array}\end{equation}This leads to the following linear equation\begin{equation}  \boxed{y^{\alpha+1}_{k+1} =  y^{\alpha}_{k+1}  -\mathcal R^{\alpha}_{yk+1}+ \\  C^{\alpha}_{k+1}(x^{\alpha+1}_{k+1}-x^{\alpha}_{k+1}) +  D^{\alpha}_{k+1}(\lambda^{\alpha+1}_{k+1}-\lambda^{\alpha}_{k+1})}. \label{eq:NL11y}\end{equation}with,\begin{equation}     \begin{array}{l}  C^{\alpha}_{k+1} = \nabla_xh(t_{k+1}, x^{\alpha}_{k+1},\lambda^{\alpha}_{k+1} ) \\ \\  D^{\alpha}_{k+1} = \nabla_{\lambda}h(t_{k+1}, x^{\alpha}_{k+1},\lambda^{\alpha}_{k+1}) \end{array}\end{equation}and\begin{equation}\fbox{$\mathcal R^{\alpha}_{yk+1} \stackrel{\Delta}{=} y^{\alpha}_{k+1} - h(x^{\alpha}_{k+1},\lambda^{\alpha}_{k+1})$} \end{equation} \paragraph{Newton's linearization of the third  line of~(\ref{eq:toto1})}The same operation is performed with the third equation of (\ref{eq:toto1})\begin{equation}  \begin{array}{l}    \mathcal R_r(r,x,\lambda)=r-g(t_{k+1},x,\lambda) =0\\ \\  \end{array}\end{equation}which is linearized as\begin{equation}  \label{eq:NL9}  \begin{array}{l}      \mathcal R_{Lr}(r^{\alpha+1}_{k+1},x^{\alpha+1}_{k+1},\lambda^{\alpha+1}_{k+1}) = \mathcal      R_{rk+1}^{\alpha} + (r^{\alpha+1}_{k+1} - r^{\alpha}_{k+1}) -      K^{\alpha}_{k+1}(x^{\alpha+1}_{k+1} - x^{\alpha}_{k+1})- B^{\alpha}_{k+1}(\lambda^{\alpha+1}_{k+1} -      \lambda^{\alpha}_{k+1})=0    \end{array}  \end{equation}\begin{equation}  \label{eq:rrL}  \begin{array}{l}    \boxed{r^{\alpha+1}_{k+1} = g(t_{k+1},x ^{\alpha}_{k+1},\lambda ^{\alpha}_{k+1}) +      K^{\alpha}_{k+1}(x^{\alpha+1}_{k+1} - x^{\alpha}_{k+1})      + B^{\alpha}_{k+1}(\lambda^{\alpha+1}_{k+1} - \lambda^{\alpha}_{k+1})    }         \end{array}\end{equation}with,\begin{equation}     \begin{array}{l}  K^{\alpha}_{k+1} = \nabla_xg(t_{k+1},x^{\alpha}_{k+1},\lambda ^{\alpha}_{k+1})  \\ \\  B^{\alpha}_{k+1} = \nabla_{\lambda}g(t_{k+1},x^{\alpha}_{k+1},\lambda ^{\alpha}_{k+1}) \end{array}\end{equation}and the  residue for $r$:\begin{equation}\boxed{\mathcal      R_{rk+1}^{\alpha} = r^{\alpha}_{k+1} - g(t_{k+1},x^{\alpha}_{k+1},\lambda ^{\alpha}_{k+1})}  \end{equation}\paragraph{Reduction to a linear relation between  $x^{\alpha+1}_{k+1}$ and $\lambda^{\alpha+1}_{k+1}$}Inserting (\ref{eq:rrL}) into~(\ref{eq:rfree-2}), we get the following linear relation between $x^{\alpha+1}_{k+1}$ and$\lambda^{\alpha+1}_{k+1}$, \begin{equation}  \label{eq:rfree-3}  \begin{array}{l}  \mathcal R^{\alpha}_{\free, k+1}  - h\gamma\left[  g(t_{k+1},x^{\alpha}_{k+1},\lambda^{\alpha}_{k+1}) +    B^{\alpha}_{k+1} (\lambda^{\alpha+1}_{k+1} - \lambda^{\alpha}_{k+1})+K^{\alpha}_{k+1}    (x^{\alpha+1}_{k+1} - x^{\alpha}_{k+1})  \right] \\  \quad\quad - h(1-\gamma)r_k  + (M-h\theta A^{\alpha}_{k+1}) (x^{\alpha+1}_{k+1} -    x^{\alpha}_{k+1})  =0  \end{array}\end{equation}that is\begin{equation}  \label{eq:rfree-4}  \begin{array}[l]{lcl}  (M-h\theta A^{\alpha}_{k+1}-h\gamma K^{\alpha}_{k+1}) (x^{\alpha+1}_{k+1}  -  x^{\alpha}_{k+1}) &=&   -  \mathcal R^{\alpha}_{\free, k+1} -h(1-\gamma) r_k \\ & & + h\gamma \left[  g(t_{k+1},x^{\alpha}_{k+1},\lambda^{\alpha}_{k+1}) +    B^{\alpha}_{k+1} (\lambda^{\alpha+1}_{k+1} - \lambda^{\alpha}_{k+1})  \right]  \end{array}\end{equation}Let us introduce some intermediate notation:\begin{equation}   \label{eq:NL9}   \begin{array}{l}     W^{\alpha}_{k+1} \stackrel{\Delta}{=} M-h\theta A^{\alpha}_{k+1}-h\gamma K^{\alpha}_{k+1})\\   \end{array} \end{equation} \begin{equation}   \label{eq:rfree-12}   \boxed{x^\alpha_{\free}\stackrel{\Delta}{=}x^{\alpha}_{k+1}-(W^{\alpha}_{k+1})^{-1}\mathcal (R_{\free,k+1}^{\alpha} \textcolor{red}{- h(1-\gamma) r_k})} \end{equation}and \begin{equation}  \boxed{x^\alpha_p \stackrel{\Delta}{=}  h\gamma(W^{\alpha}_{k+1} )^{-1}\left[g(t_{k+1},x^{\alpha}_{k+1},\lambda^{\alpha}_{k+1})     -B^{\alpha}_{k+1} (\lambda^{\alpha}_{k+1}) \right ] +x^\alpha_{\free}}.\end{equation}The relation (\ref{eq:rfree-4}) can be written as\begin{equation}  \label{eq:rfree-13}  \begin{array}{l}    \boxed{   x^{\alpha+1}_{k+1}\stackrel{\Delta}{=}  x^\alpha_p +  \left[ h \gamma (W^{\alpha}_{k+1})^{-1}    B^{\alpha}_{k+1} \lambda^{\alpha+1}_{k+1}\right]}   \end{array}\end{equation}\paragraph{Reduction to a linear relation between  $y^{\alpha+1}_{k+1}$ and$\lambda^{\alpha+1}_{k+1}$.}Inserting (\ref{eq:rfree-13}) into (\ref{eq:NL11y}), we get the following linear relation between $y^{\alpha+1}_{k+1}$ and $\lambda^{\alpha+1}_{k+1}$, \begin{equation}   \begin{array}{l}     y^{\alpha+1}_{k+1} = y_p + \left[ h \gamma C^{\alpha}_{k+1} ( W^{\alpha}_{k+1})^{-1}  B^{\alpha}_{k+1} + D^{\alpha}_{k+1} \right]\lambda^{\alpha+1}_{k+1}   \end{array}\end{equation}with \begin{equation}\boxed{    y_p = y^{\alpha}_{k+1} -\mathcal R^{\alpha}_{yk+1} + C^{\alpha}_{k+1}(x_q) -   D^{\alpha}_{k+1} \lambda^{\alpha}_{k+1} }\end{equation}\textcolor{red}{  \begin{equation}   \boxed{ x_q=x^\alpha_p -x^{\alpha}_{k+1}\label{eq:xqq}}  \end{equation}}% \paragraph{With $\gamma =1$:}% \[(W^{\alpha}_{k+1} )x^{\alpha+1}_{k+1}= hr^{\alpha+1}_{k+1}- \mathcal R_{\free, k+1} ^{\alpha}+W^{\alpha}_{k+1}x^{\alpha}_{k+1}\]% \[x^{\alpha+1}_{k+1}= h( W^{\alpha}_{k+1})^{-1}r^{\alpha+1}_{k+1}-% ( W^{\alpha}_{k+1})^{-1} \mathcal R_{\free k+1} ^{\alpha}+x^{\alpha}_{k+1}\]% \[x^{\alpha+1}_{k+1}= h( W^{\alpha}_{k+1})^{-1}r^{\alpha+1}_{k+1}+x_{\free}\]% with, using \ref{}% \begin{equation}% x_p-x^{\alpha}_{k+1}=h(% W^{\alpha}_{k+1})^{-1}(g(x^{\alpha}_{k+1},\lambda^{\alpha}_{k+1},t_{k+1})-B^{\alpha}_{k+1}% \lambda^{\alpha}_{k+1}-K^{\alpha}_{k+1} x^{\alpha}_{k}))+\tilde x_{\free}% \end{equation}% \[    \tilde x_{\free}= -( W^{\alpha}_{k+1})^{-1} \mathcal R _{\free k+1} ^{\alpha} \]%       \[x_{\free} = \tilde x_{\free} + x^{\alpha}_{k+1}=\fbox{$- W^{-1}R_{\free k+1} ^{\alpha} + x^{\alpha}_{k+1}$}\]% \[ \fbox{$x_p  = x_{\free} + h ( W^{\alpha}_{k+1})^{-1}( g(x ^{\alpha}_{k+1},\lambda ^{\alpha}_{k+1},t_{k+1}) -%       B^{\alpha}_{k+1} \lambda^{\alpha}_{k+1}-K^{\alpha}_{k+1} x^{\alpha}_{k+1} )$} \]\paragraph{Mixed linear complementarity problem (MLCP)}To summarize, the problem to be solved in each Newton iteration is:\\{  \begin{minipage}[l]{1.0\linewidth}    \begin{equation}      \begin{cases}      \begin{array}[l]{l}        y^{\alpha+1}_{k+1} =   W_{mlcpk+1}^{\alpha}  \lambda^{\alpha+1}_{k+1} + b^{\alpha}_{k+1}        \\ \\        -y^{\alpha+1}_{k+1} \in N_{[l,u]}(\lambda^{\alpha+1}_{k+1} ).       \end{array}      \label{eq:NL14}      \end{cases}    \end{equation}  \end{minipage}}with $W_{mlcpk+1}\in \RR^{m\times m}$ and $b\in\RR^{m}$ defined by\begin{equation}  \label{eq:NL15} \begin{array}[l]{l}   W_{mlcpk+1}^{\alpha} = h \gamma C^{\alpha}_{k+1}  (W^{\alpha}_{k+1})^{-1}  B^{\alpha}_{k+1} + D^{\alpha}_{k+1} \\   b^{\alpha}_{k+1} = y_p\end{array}\end{equation}The problem~(\ref{eq:NL14}) is equivalent to a Mixed Linear Complementarity Problem (MLCP) which can be solved under suitable assumptions by many linear complementarity solvers such as pivoting techniques, interior point techniques and splitting/projection strategies. The  reformulation into a standard MLCP follows the same line as for the MCP in the previous section. One obtains,    \begin{equation}      \begin{array}[l]{l}        y^{\alpha+1}_{k+1} =   - W^{\alpha}_{k+1}  \lambda^{\alpha+1}_{k+1} + b^{\alpha}_{k+1}        \\ \\        (y^{\alpha+1}_{k+1})_i  = 0 \qquad \textrm{ for } i \in \{ 1..n\}\\[2mm]        0 \leq  (\lambda^{\alpha+1}_{k+1})_i\perp (y^{\alpha+1}_{k+1})_i \geq 0 \qquad \textrm{ for } i \in \{ n..n+m\}\\      \end{array}      \label{eq:MLCP1}     \end{equation}%%% Local Variables: %%% mode: latex%%% TeX-master: "DevNotes"%%% End: